Add some things

src/pregeom/basic.lean
@@ -1,17 +1,108 @@
 import data.finset
 
+open_locale classical
+
 variable (T : Type*)
 
 class has_cl :=
 (cl : set T → set T)
 
+open has_cl
 open has_insert
 
 class inf_pregeom extends has_cl T :=
-(inclusion {S} : S ⊆ cl S)
+(inclusive {S} : S ⊆ cl S)
 (monotone {S1 S2} : S1 ⊆ S2 → cl S1 ⊆ cl S2)
 (idempotent {S} : cl (cl S) = cl S)
 (exchange {x y} {S} : x ∈ cl (insert y S) → x ∉ cl S → y ∈ cl (insert x S))
 
 class pregeom extends inf_pregeom T := 
 (finchar {x} {S} : x ∈ cl S → ∃ U : finset T, ↑U ⊆ S ∧ x ∈ cl ↑U)
+
+namespace has_cl
+
+lemma reg_set_incl [has_cl T] {S : set T} : {t : T | t ∉ cl (∅ : set T)} ∩ S ⊆ S := by exact {t : T | t ∉ cl ∅}.inter_subset_right S
+
+end has_cl
+
+namespace inf_pregeom 
+variable [inf_pregeom T]
+variable {T}
+
+lemma mem_cl_of_subset_mem {x : T} {A B : set T} : A ⊆ B → x ∈ cl A → x ∈ cl B := 
+begin
+  intros h hx,
+  exact inf_pregeom.monotone h hx,
+end
+
+lemma cl_union_cl_subset_cl_union {A B : set T} : cl A ∪ cl B ⊆ cl (A ∪ B) :=
+begin
+  intros s hs,
+  cases hs,
+  {
+    have : A ⊆ A ∪ B, by exact set.subset_union_left A B,
+    exact monotone this hs,
+  },
+  {
+    have : B ⊆ A ∪ B, by exact set.subset_union_right A B,
+    exact monotone this hs,
+  },
+end
+
+@[simp]
+lemma cl_cl_union {A B : set T} : cl (cl A ∪ B) = cl (A ∪ B) := 
+begin
+  ext,
+  split,
+  {
+    intro h,
+    rw ←idempotent,
+    have : cl A ∪ B ⊆ cl (A ∪ B),
+    {
+      intros t ht,
+      cases ht,
+      {
+        have : A ⊆ A ∪ B, by exact set.subset_union_left A B,
+        replace this := monotone this,
+        apply this,
+        assumption,
+      },
+      {
+        have : B ⊆ A ∪ B, by exact set.subset_union_right A B,
+        replace this := monotone this,
+        apply this, apply inclusive, assumption,
+      }
+    },
+    replace this := monotone this,
+    apply this,
+    assumption,
+  },
+  {
+    have : A ∪ B ⊆ cl A ∪ B, by exact set.union_subset_union_left B inclusive,
+    intro h,
+    exact monotone this h,
+  }
+end
+
+@[simp]
+lemma cl_union_cl {A B : set T} : cl (A ∪ cl B) = cl (A ∪ B) := 
+begin
+  have : A ∪ cl B = cl B ∪ A, by exact sup_comm, rw this,
+  have : A ∪ B = B ∪ A, by exact sup_comm, rw this,
+  exact cl_cl_union
+end
+
+@[simp]
+lemma cl_cl_union_cl {A B : set T} : cl (cl A ∪ cl B) = cl (A ∪ B) := 
+calc cl (cl A ∪ cl B) = cl (cl A ∪ B) : cl_union_cl
+... = cl (A ∪ B) : cl_cl_union
+
+@[simp]
+lemma cl_empty_union [inf_pregeom T] {S : set T} :
+  cl (cl (∅ : set T) ∪ S) = cl S := 
+calc cl (cl (∅ : set T) ∪ S) = cl (cl ∅ ∪ cl S) : by rw ←cl_union_cl
+... = cl (∅ ∪ cl S) : by rw cl_cl_union
+... = cl (cl S) : by rw set.empty_union
+... = cl S : by rw inf_pregeom.idempotent
+
+end inf_pregeom
