src/pregeom/regularize.lean
@@ -1,0 +1,117 @@
+import .basic
+import data.finset
+
+open_locale classical
+
+open has_cl
+
+variable (T : Type*)
+
+def reg_set [has_cl T] := {t : T | t ∉ cl (∅ : set T) }
+def reg [has_cl T] := subtype (reg_set T)
+
+namespace reg
+
+open inf_pregeom
+variable {T}
+
+local notation `ι` := subtype.val
+
+instance has_cl [has_cl T] : has_cl (reg T) :=
+⟨ λ S, ι ⁻¹' cl (ι '' S) ⟩ 
+
+@[simp]
+lemma mem_cl_iff_val_mem_cl [has_cl T] {x : reg T} {S : set (reg T)} : x ∈ cl S ↔ x.val ∈ cl (ι '' S) := by trivial
+
+@[simp]
+lemma image_cl_eq_cl_reg_image [has_cl T] {S : set (reg T)} : 
+  ι '' (cl S : set (reg T)) = reg_set T ∩ cl (ι '' S) :=
+begin
+  ext s, split,
+  {
+    rintro ⟨s', h1, h2⟩,
+    rw ←h2, 
+    exact ⟨s'.2, h1⟩
+  },
+  {
+    rintro ⟨h1,h2⟩,
+    use ⟨s, h1⟩,
+    split,
+    exact h2,
+    simp only [],
+  },
+end
+
+@[simp]
+theorem cl_reg_inter [inf_pregeom T] {S : set T} :
+  cl (reg_set T ∩ S) = cl S :=
+begin
+  ext, split,
+  { 
+    have : reg_set T ∩ S ⊆ S, by exact reg_set_incl T,
+    apply monotone this,
+  },
+  {
+    intro h,
+    have : reg_set T ∩ S = ∅ ∪ (reg_set T ∩ S), by finish,
+    rw [this, ←cl_cl_union],
+    have : S ⊆ cl ∅ ∪ reg_set T ∩ S,
+    {
+      intros s hs,
+      by_cases s ∈ cl (∅ : set T),
+      left, assumption,
+      right, split; assumption,
+    }, 
+    apply monotone this,
+    assumption,
+  }
+end
+
+instance inf_pregeom [inf_pregeom T] : inf_pregeom (reg T) := 
+begin
+  split; intros,
+  {
+    intros s hs,
+    rw mem_cl_iff_val_mem_cl,
+    have : s.val ∈ ι '' S, by exact set.mem_image_of_mem ι hs,
+    exact inclusive this,
+  },
+  {
+    intros s hs,
+    rw mem_cl_iff_val_mem_cl at *,
+    have : ι '' S1 ⊆ ι '' S2, by exact set.image_subset ι a,
+    apply monotone this,
+    assumption,
+  },
+  {
+    ext, split,
+    repeat {
+      intro hx,
+      rw [mem_cl_iff_val_mem_cl,image_cl_eq_cl_reg_image,cl_reg_inter,idempotent] at *,
+      assumption,
+    },
+  },
+  {
+    rw mem_cl_iff_val_mem_cl,
+    have : ι '' insert x S = insert x.val (ι '' S), by exact set.image_insert_eq, rw this,
+    apply exchange,
+    rw ←set.image_insert_eq, 
+    assumption'
+  }
+end
+
+instance pregeom [pregeom T] : pregeom (reg T) := 
+begin
+  split, intros x S hx,
+  cases x with x h,
+  have : x ∈ cl (ι '' S),
+  {
+    rw mem_cl_iff_val_mem_cl at hx,
+    simpa only [],
+  },
+  cases pregeom.finchar this with W hW,
+  -- we need the statement that the preimage of a finite set under an injective map is a finite set.
+  sorry,
+end
+
+end reg
